---
layout: post
title: Eigenvalue and EigenVector
tags: eigenvalue, eigenvector, decomposition, basic
math: true
date: 2024-08-24 15:32 +0800
---

# Definition of Eigenvalue & Eigenvector

$$
Av = \lambda v 
$$
For square matrix \\\(A\\\), we can see this matrix as linear transformation for vector \\\(v\\\), where \\\(v\\\) does not equal to 0. We call this 'eigenvector', with constant multiplication value called 'eigenvalue'.

$$
\left(\begin{array}{ccc} 
a_{11} & a_{12} & a_{13}\\
a_{21} & a_{22} & a_{23}\\
a_{31} & a_{32} & a_{33}\\
\end{array}\right)
\left(\begin{array}{c} 
v_1\\ 
v_2\\
v_3
\end{array}\right)
=
\lambda
\left(\begin{array}{c}
v_1\\
v_2\\
v_3
\end{array}\right)
$$ 

That is, \\\(\lambda\\\) implies eigenvalue of matrix \\\(A\\\), and \\\(v\\\) implies eigenvector of matrix $A$ in terms of \\\(\lambda\\\). Direction of vector \\\(v\\\) did not change, only amount of magnitude did as much as \\\(\lambda\\\) after linear transformation $A$.

As \\\((A - \lambda I)v = 0\\\), inverse matrix of \\\(A - \lambda I\\\) cannot exists. (if exists, \\\(v\\\) becomes 0 that violates our assumption.) Therefore, 
$$
det(A - \lambda I) = 0
$$


Apply it on real numberset
$$
A 
= 
\left(\begin{array}{cc}
1 & 2 \\
2 & 4
\end{array}\right)
$$

since, 
$$
det(A - \lambda I) = 0 \\
\\
det\left(\begin{array}{cc}
1-\lambda & 2 \\
2 & 4-\lambda
\end{array}\right)
=0
$$

$$
(1-\lambda)*(4-\lambda) - 4 = 0 \\
\lambda^2 - 5 \lambda = 0 \\
$$

$\therefore \ \lambda = 0, 5$

When \\\(\lambda = 0\\\),
$$
\left(\begin{array}{cc}
1 & 2 \\
2 & 4 
\end{array}\right)
\left(\begin{array}{cc}
v_1 \\
v_2
\end{array}\right) = 0
$$
\\\(v_1 + 2 v_2 = 0\\\) and \\\(2 v_1 + 4 v_2 = 0\\\)
Therefore, \\\(v_1 = - v_2\\\) which shows matrix A dimension is lower than 2.

When \\\(\lambda = 5\\\),
$$
\left(\begin{array}{cc}
1 & 2 \\
2 & 4
\end{array}\right)
\left(\begin{array}{cc}
v_1 \\
v_2
\end{array}\right) = 
5
\left(\begin{array}{cc}
v_1 \\
v_2
\end{array}\right)
$$
\\\(v_1 + 2 v_2 = 5 v_1\\\) and \\\(2 v_1 + 4 v_2 = 5 v_2\\\)
Therefore, \\\(v_2 = 2 v_1\\\) for eigenvalue \\\(\lambda = 5\\\).

We can do EigenDecomposition using above ideas.


reference : https://darkpgmr.tistory.com/105


## Examples

Example 5.8 from Axler, S. (2015). Linear algebra done right (3rd ed.). New York, NY: Springer


Suppose \\\(T \in \mathcal{L}\left(\mathbf{F}^2\right)\\\) is defined by

$$
T(w, z)=(-z, w) .
$$

(a) Find the eigenvalues and eigenvectors of \\\(T\\\) if \\\(\mathbf{F}=\mathbf{R}\\\).

(b) Find the eigenvalues and eigenvectors of \\\(T\\\) if \\\(\mathbf{F}=\mathbf{C}\\\).


solution (a) \
If \\\(\mathbf{F}=\mathbf{R}\\\), then \\\(T\\\) is a counterclockwise rotation by \\\(90^{\circ}\\\) about the origin in \\\(\mathbf{R}^2\\\). \\\(T(w, z)=(-z, w)\\\) \
An operator \\\(T\\\) has an eigenvalue if and only if there exists a nonzero vector in its domain that gets sent by the operator to a scalar multiple of itself. However, \\\(90^{\circ}\\\) counterclockwise rotation of a nonzero vector in \\\(\mathbf{R}^2\\\) obviously never equals a scalar multiple of itself.  
Conclusion: if \\\(\mathbf{F}=\mathbf{R}\\\), then \\\(T\\\) has no eigenvalues (and thus has no eigenvectors).



solution (b) \
To find eigenvalues of \\\(T\\\), we must find the scalars \\\(\lambda\\\) such that

$$
T(w, z)=\lambda(w, z) = (-z, w)
$$

has some solution other than \\\(w=z=0\\\). The equation above is equivalent to the simultaneous equations.

$$
-z=\lambda w, \quad w=\lambda z .
$$


Substituting the value for $w$ given by the second equation into the first equation gives

$$
-z=\lambda^2 z
$$


Now \\\(z\\\) cannot equal 0, so the equation above leads to the equation

$$
-1=\lambda^2 \\
$$

\\\(\therefore \lambda = \plusmn i\\\)

It is easy to verify that \\\(i\\\) and \\\(-i\\\) are eigenvalues of \\\(T\\\). Indeed, the eigenvectors corresponding to the eigenvalue \\\(i\\\) are the vectors of the form \\\((w,-w i)\\\), with \\\(w \in \mathbf{C}\\\) and \\\(w \neq 0\\\), and the eigenvectors corresponding to the eigenvalue \\\(-i\\\) are the vectors of the form \\\((w, w i)\\\), with \\\(w \in \mathbf{C}\\\) and \\\(w \neq 0\\\). (Multiplication of \\\(i^3\\\) and \\\(i\\\) for the equation \\\(\lambda(w, z) = (-z, w)\\\))